Dafny/BloodInventory.dfy
@@ -2,12 +2,42 @@ include "Blood.dfy"
 class BloodInventory
 {
     var bloodInventory: array<Blood>;
+    var bloodInventoryCover: array<string>;
     var threshold: int;
     var alert: bool;
 
     predicate Valid()
     reads this
+    requires bloodInventoryCover != null
     {
-        
+        alert ==> (threshold >= CountByBloodType("A+")) 
     } 
+
+    // function CountByBloodType(bloodType:string): int
+    // requires bloodInventoryCover != null
+    // reads this
+    // ensures CountByBloodType(bloodType) == CheckIndexForBloodType(bloodType,  bloodInventoryCover.Length - 1)
+    // {
+    //     CheckIndexForBloodType(bloodType,  bloodInventoryCover.Length - 1)
+    // }
+
+    // function CheckIndexForBloodType(bloodType: string, index: int): int
+    // requires bloodInventoryCover != null
+    // requires index < bloodInventoryCover.Length
+    // reads this
+    // decreases index
+    // ensures (index < 0) ==> (CheckIndexForBloodType(bloodType, index) == 0)
+    // ensures (index >= 0 && (bloodInventoryCover[index] == bloodType)) ==> (CheckIndexForBloodType(bloodType, index) == CheckIndexForBloodType(bloodType, index - 1) + 1) 
+    // ensures (index >= 0 && (bloodInventoryCover[index] != bloodType)) ==> (CheckIndexForBloodType(bloodType, index) == CheckIndexForBloodType(bloodType, index - 1)) 
+    // {
+    //     if index < 0 
+    //     then
+    //         0
+    //     else
+    //         if bloodInventoryCover[index] == bloodType
+    //         then
+    //             CheckIndexForBloodType(bloodType, index - 1) + 1
+    //         else
+    //             CheckIndexForBloodType(bloodType, index - 1)
+    // }
 } // end of BloodInventory class
